Add a filesystem semantics
Used a few combinators for building relations to write a reasonably
clean semantics, including all the error cases.

src/Database/Filesys.v
@@ -1,9 +1,28 @@
 From RecoveryRefinement Require Import Lib.
 From RecoveryRefinement Require Import Helpers.MachinePrimitives.
+From RecoveryRefinement Require Import Helpers.RelationAlgebra.
+
+From Classes Require Import EqualDec.
+Import EqualDecNotation.
+
+From stdpp Require gmap.
+From stdpp Require Import fin_maps.
 
 From Coq Require Import String.
 
 Definition Path := string.
+
+Instance ascii_eqdec : EqualDec Ascii.ascii.
+hnf.
+decide equality; decide equality.
+Defined.
+
+(* TODO: add this instance to coq-classes *)
+Instance path_eqdec : EqualDec Path.
+hnf.
+decide equality.
+destruct (equal a a0); auto.
+Defined.
 
 Module FS.
   Implicit Types (p:Path) (fh:Fd) (bs:ByteString).
@@ -32,4 +51,79 @@ Module FS.
   Definition delete p := Call (Delete p).
   Definition truncate fh := Call (Truncate fh).
   Definition atomicCreate p bs := Call (AtomicCreate p bs).
+
+  Inductive OpenMode := Read | Write.
+
+  Instance mode_eqdec : EqualDec OpenMode := ltac:(hnf; decide equality).
+
+  Record State :=
+    { files: gmap Path ByteString;
+      fds: gmap Fd (Path * OpenMode); }.
+
+  Definition upd_files (f: _ -> _) (s:State) : State :=
+    {| files := f s.(files);
+       fds := s.(fds); |}.
+
+  Definition upd_fds (f: _ -> _) (s:State) : State :=
+    {| files := s.(files);
+       fds := f s.(fds); |}.
+
+  Definition readFd (fh: Fd) (m: OpenMode) : relation State State Path :=
+    readSome (fun s => match s.(fds) !! fh with
+                    | Some (p, m') => if m == m' then Some p else None
+                    | _ => None
+                    end).
+
+  Import RelationNotations.
+
+  Definition step T (op:Op T) : relation State State T :=
+    (* NOTE: dependent match annotations improve error messages (the error
+    message can now include the expected type T based on branch) *)
+    match op in Op T return relation State State T with
+    | Open p =>
+      _ <- readSome (fun s => s.(files) !! p);
+        fh <- such_that (fun s fh => s.(fds) !! fh = None);
+        _ <- puts (upd_fds (insert fh (p, Read)));
+        pure fh
+    | Close fh =>
+      puts (upd_fds (map_delete fh))
+    | List =>
+      reads (fun s => map fst (map_to_list s.(files)))
+    | Size fh =>
+        bs <- (p <- readFd fh Read;
+                readSome (fun s => s.(files) !! p));
+        pure (BS.length bs)
+    | ReadAt fh off len =>
+      p <- readFd fh Read;
+        bs <- (p <- readFd fh Read;
+                readSome (fun s => s.(files) !! p));
+        pure (BS.take len (BS.drop off bs))
+    | Create p =>
+      fh <- such_that (fun s fh => s.(fds) !! fh = None);
+        _ <- readNone (fun s => s.(files) !! p);
+        _ <- puts (upd_files (insert p BS.empty));
+        _ <- puts (upd_fds (insert fh (p, Write)));
+        pure fh
+    | Append fh bs' =>
+      p <- readFd fh Write;
+        bs <- readSome (fun s => s.(files) !! p);
+        puts (upd_files (insert p (BS.append bs bs')))
+    | Delete p =>
+      (* Delete(p) fails if there is an open fh pointing to p - this is a safe
+      approximation of real behavior, where the underlying inode for the file is
+      retained as long as there are open files *)
+      (_ <- such_that (fun s fh =>
+                        exists m, s.(fds) !! fh = Some (p, m)); error)
+      (* delete's error case supercedes this succesful deletion case *)
+      + puts (upd_files (map_delete p))
+    | Truncate fh =>
+      p <- (p <- readFd fh Write;
+             _ <- readSome (fun s => s.(files) !! p);
+             pure p);
+        puts (upd_files (insert p BS.empty))
+    | AtomicCreate p bs =>
+      _ <- readNone (fun s => s.(files) !! p);
+        puts (upd_files (insert p bs))
+    end.
+
 End FS.
